src/program_proof/simplefs/bitmap_byte.v
@@ -1,0 +1,63 @@
+From stdpp Require Import base numbers list_numbers.
+From Coq Require Import ssreflect.
+From Perennial.Helpers Require Import Integers.
+From Perennial.Helpers Require Import bytes.
+
+Import Coq.Init.Nat.
+
+#[local] Open Scope Z.
+
+(* This file contains two proofs that are done by exploding all cases (eg, all
+256 values for a [w8]). These proofs are rather slow (roughly 20s), so they make
+iterating on the main bitmap tedious. *)
+
+Lemma split_div_mod_8 (i: nat) :
+  ∃ (i1 i2: nat),
+    (i `div` 8 = i1 ∧
+    i `mod` 8 = i2 ∧
+    i = 8 * i1 + i2 ∧
+    8 * i1 ≤ i ∧
+    0 ≤ i2 < 8)%nat.
+Proof.
+  eexists _, _; split_and!; [ eauto | eauto | .. ].
+  - rewrite {1}(Nat.div_mod i 8) //.
+  - apply Nat.Div0.mul_div_le; lia.
+  - apply Nat.mod_bound_pos; lia.
+  - apply Nat.mod_bound_pos; lia.
+Qed.
+
+Lemma Some_inv {A} (a b: A) : Some a = Some b → a = b.
+Proof. inversion 1; auto. Qed.
+
+Lemma Some_eq_iff {A} (a b: A) : Some a = Some b ↔ a = b.
+Proof. split; [ apply Some_inv | congruence ]. Qed.
+
+Local Ltac Zify.zify_post_hook ::= Z.div_mod_to_equations.
+
+Transparent w8_instance.w8.
+Lemma set_bit_get (b: w8) (i: u64) bit :
+  byte_to_bits (word.or b (word.slu (W8 1) (W8 (uint.Z i `mod` 8))))
+  !! Z.to_nat (uint.Z i `mod` 8) = Some bit → true = bit.
+Proof.
+    byte_cases b; bit_off_cases (uint.Z i `mod` 8);
+      intros H%Some_inv; exact H.
+Qed.
+Opaque w8_instance.w8.
+
+Opaque Nat.div Nat.modulo.
+
+Lemma testbit_set_bit (b: w8) (i: Z) (i': nat) :
+  0 ≤ i < 8 →
+  (i' < 8)%nat →
+  Z.testbit (uint.Z (word.or b (word.slu (W8 1) (W8 i)))) (Z.of_nat i') =
+  if decide (i = Z.of_nat i') then true else Z.testbit (uint.Z b) (Z.of_nat i').
+Proof.
+  intros Hbound Hbound'.
+  (* this order is slightly faster than doing all the destructs first (it
+  computes the decide first) *)
+  bit_off_cases i; bit_off_cases i';
+    simpl;
+    byte_cases b;
+    vm_compute;
+    try reflexivity.
+Qed.
